theories/Misc.v
@@ -1,0 +1,45 @@
+From ConCert Require Import CustomTactics.
+From MetaCoq Require Import utils.
+Require Import List.
+
+
+Lemma forallb_Forall_iff {A} (p : A -> bool) (l : list A):
+  Forall (fun x => p x = true) l <-> forallb p l = true.
+Proof.
+  split.
+  + induction l;intros H.
+    * reflexivity.
+    * simpl. inversion H as [H1 | a1 l1 Heq]. subst. rewrite Heq. simpl.
+      now eapply IHl.
+  + induction l;intros H.
+    * constructor.
+    * simpl in *. rewrite Bool.andb_true_iff in *. destruct H.
+      constructor;auto.
+Qed.
+
+Lemma Forall_impl_inner {A} (P Q : A -> Prop) l :
+  Forall P l -> Forall (fun x => P x -> Q x) l ->
+  Forall Q l.
+Proof.
+  intros HP. induction HP;intros HQ.
+  + constructor.
+  + constructor;inversion HQ;auto.
+Qed.
+
+
+Lemma All_impl_inner {A} (P Q : A -> Type) l :
+  All P l -> All (fun x => P x -> Q x) l ->
+  All Q l.
+Proof.
+  intros HP. induction HP;intros HQ.
+  + constructor.
+  + constructor;inversion HQ;auto.
+Qed.
+
+Lemma forallb_impl_inner {A} {p q} {l : list A} :
+  forallb p l -> (forall x, p x = true -> q x = true) -> forallb q l.
+Proof.
+  revert p q.
+  induction l;simpl;intros p q Hfa H;auto.
+  inv_andb Hfa. split_andb;try eapply IHl;eauto.
+Qed.
